snapshot progress

Examples/Snapshot.v
@@ -3,6 +3,7 @@ From LHL.Core Require Import
   LogicFacts
   SingConds
   Program
+  ProgramFacts
   VisPoss
   Tensor
   Traces
@@ -19,6 +20,11 @@ From LHL.Util Require Import
   TransUtil
   Tactics
   Util.
+
+From Coq Require Import
+  Logic.PropExtensionality
+  Logic.FunctionalExtensionality
+  Unicode.Utf8.
 
 Record reg_st {A} := {
   val : option A;
@@ -44,7 +50,13 @@ Notation valSt s i := (
   end
 ).
 
-Notation ranSt s i := (
+Notation oranSt ρ i := (
+  match ρ.(PState) with
+  | SnapDef _ _ c => c i
+  end
+).
+
+Notation uranSt s i := (
   match RState (snd s) i with
   | RegDef s _ => s.(ran)
   end
@@ -56,40 +68,47 @@ Notation snapSt x := (
   end
 ).
 
+Notation pendSt x := (
+  match PState x with
+  | SnapDef s _ _ => s
+  end
+).
+
+Notation "` x" := (proj1_sig x) (at level 40).
+
 Definition StateM E A R :=
   A -> Prog E (R * A).
 
-Definition runStateM {E A R} (a : A) (m : StateM E A R) : Prog E R :=
-  p <- m a;
-  ret (fst p).
+Definition runStateM {E A R} (a : A) (m : StateM E A R) : Prog E (R * A) :=
+  m a.
 
 Definition get {E A} : StateM E A A :=
-  fun a => ret (a, a).
+  λ a, ret (a, a).
 
 Definition put {E A} (s : A) : StateM E A unit :=
-  fun _ => ret (tt, s).
+  λ _, ret (tt, s).
 
 Definition upd {E A} (f : A -> A) : StateM E A unit :=
-  fun s => ret (tt, f s).
+  λ s, ret (tt, f s).
 
 Definition bindM {E A B C}
   (m : StateM E A B)
   (k : B -> StateM E A C)
 : StateM E A C :=
-  fun s =>
+  λ s,
     p <- m s;
     k (fst p) (snd p).
 
 Definition retM {E A R} (x : R) : StateM E A R :=
-  fun s => ret (x, s).
+  λ s, ret (x, s).
 
 Definition lift {E A R} (p : Prog E R) : StateM E A R :=
-  fun s =>
+  λ s,
     r <- p;
     ret (r, s).
 
-Notation "x <- f ;' m" := (bindM f (fun x => m)) (at level 80, right associativity).
-Notation "f ;;' m" := (bindM f (fun _ => m)) (at level 80, right associativity).
+Notation "x <- f ;' m" := (bindM f (λ x, m)) (at level 80, right associativity).
+Notation "f ;;' m" := (bindM f (λ _, m)) (at level 80, right associativity).
 
 Section while.
 
@@ -103,7 +122,7 @@ CoFixpoint whileAux (e' : Prog E (unit * A)) : Prog E (unit * A) :=
     else
       ret (tt, t)
   | Bind m k =>
-    Bind m (fun x => whileAux (k x))
+    Bind m (λ x, whileAux (k x))
   | NoOp e' => NoOp (whileAux e')
   end.
 
@@ -111,11 +130,133 @@ Definition while s := NoOp (whileAux (e s)).
 
 End while.
 
-Fixpoint range {E A} (n : nat) (e : nat -> StateM E A unit) : StateM E A unit :=
+Require Import Lia.
+
+Program Fixpoint range {E A} (n : nat) (e : Index n -> StateM E A unit) : StateM E A unit :=
   match n with
   | 0 => retM tt
   | S n => e n ;;' range n e
   end.
+Next Obligation.
+  destruct x.
+  cbn. lia.
+Qed.
+
+Program Definition wkIx {N} (i : Index N) : Index (S N) := i.
+Next Obligation.
+  destruct i.
+  cbn. lia.
+Qed.
+
+Section control_lemmas.
+
+Context
+  {T : nat} {E F : ESig}
+  {VE : Spec T E} {VF : Spec T F}
+  {R G : Relt VE VF}.
+
+Lemma lemRange {A} {i : Name T} :
+  ∀ (N : nat) (e : Index N -> StateM E A unit)
+    (I : nat -> A -> Relt VE VF),
+    (∀ n s,
+      ∀ p : n < N,
+      VerifyProg i R G
+        (I (S n) s)
+        (runStateM s (e (exist _ n p)))
+        (λ '(tt, t), I n t)) ->
+    ∀ s,
+      VerifyProg i R G
+        (I N s)
+        (runStateM s (range N e))
+        (λ r, I 0 (snd r)).
+Proof.
+  intros N e I H.
+  induction N;
+  cbn; intros s.
+  { now constructor. }
+  {
+    eapply lemBind.
+    { apply H. }
+    {
+      intros [[] t]. simpl in *.
+      apply IHN. intros. apply H.
+    }
+  }
+Qed.
+
+End control_lemmas.
+
+Program Definition zeroIx {N} : Index (S N) := 0.
+Next Obligation. lia. Qed.
+
+Lemma mret_lid {E A} :
+  ∀ e : StateM E A unit,
+    (retM tt;;' e) = e.
+Proof.
+Admitted.
+
+Lemma mret_rid {E A} :
+  ∀ e : StateM E A unit,
+    (e;;' retM tt) = e.
+Proof.
+Admitted.
+
+Lemma range_unfold {E A n} {e : Index (S n) -> StateM E A unit} :
+  range (S n) e = (range n (λ i, e (wkIx i)) ;;' e zeroIx).
+induction n; cbn in *.
+{
+  rewrite mret_lid, mret_rid.
+  unfold zeroIx. do 2 f_equal.
+  apply proof_irrelevance.
+}
+{
+  admit.
+}
+Admitted.
+
+Lemma ret_lunit {E A B} :
+  ∀ (v : A) (k : A -> Prog E B),
+    (x <- ret v; k x) = k v.
+Proof.
+  intros v k.
+  rewrite frobProgId at 1.
+  simpl. now destruct (k v).
+Qed.
+
+CoInductive coeq {A} (x : A) : A -> Prop :=
+| coeq_refl : coeq x x.
+
+Lemma coeq_eq {A} :
+  ∀ x y : A,
+    coeq x y <-> eq x y.
+Proof.
+  intros x y.
+  split; now intros [].
+Qed.
+
+Lemma ret_runit {E A} :
+  ∀ e : Prog E A,
+    bindProg e ret = e.
+Proof.
+  (* assert (∀ e : Prog E A, coeq (bindProg e ret) e).
+  {
+    cofix rec. intros e.
+    rewrite frobProgId at 1.
+    destruct e; simpl.
+    {
+      rewrite coeq_eq. f_equal.
+      extensionality x.
+      rewrite <- coeq_eq.
+      apply rec.
+    }
+    { constructor. }
+    {
+      rewrite coeq_eq. f_equal.
+      rewrite <- coeq_eq. apply rec.
+    }
+  }
+  now setoid_rewrite <- coeq_eq. *)
+Admitted.
 
 Definition prop (P : Prop) : bool :=
   if classicT P then true else false.
@@ -135,34 +276,49 @@ Record loop_st {A} := {
 }.
 Arguments loop_st : clear implicits.
 
+Definition fill_old {A} T : StateM (E T A) (loop_st A) unit :=
+  range T (λ i,
+    v <- lift (call (At i Read));'
+    s <- get;'
+    match v.(val) with
+    | Some v => put {| old := insert v s.(old); new := s.(new)|}
+    | None => retM tt
+    end
+  ).
+
+Definition fill_new {A} T : StateM (E T A) (loop_st A) unit :=
+  range T (λ i,
+    v <- lift (call (At i Read));'
+    s <- get;'
+    match v.(val) with
+    | Some v => put {| old := s.(old); new := insert v s.(new)|}
+    | None => retM tt
+    end
+  ).
+
 (* fst is old, snd is new *)
 Definition write_snapshot {T A} (v : A) : Prog (E T A) (option (set A)) :=
   i <- call Self;
-  let i := proj1_sig i in
   st <- call (At i Read);
   if st.(ran) then
     ret None
   else
     call (At i (Write {| val := Some v; ran := true |}));;
-    runStateM {| old := emp; new := emp |} (
-      while (fun s => prop (s.(new) <> s.(old))) (
+    res <- runStateM {| old := emp; new := emp |} (
+      fill_old T;;'
+      fill_new T;;'
+      while (λ s, negb (s.(new) =? s.(old))) (
         s <- get;'
         put {| old := s.(new); new := emp |};;'
-        range T (fun i =>
-          v <- lift (call (At i Read));'
-          s <- get;'
-          match v.(val) with
-          | Some v => put {| old := s.(old); new := insert v s.(new)|}
-          | None => retM tt
-          end
-        )
+        fill_new T
       );;'
       s <- get;'
       retM (Some s.(new))
-    ).
+    );
+    ret (fst res).
 
 Definition snapImpl T A : Impl (E T A) (SnapSig A) :=
-  fun _ m => match m with
+  λ _ m, match m with
   | WriteSnap v => write_snapshot v
   end.
 
@@ -173,50 +329,195 @@ Notation "x ⊆ y" :=
   (forall v, v ∈ x -> v ∈ y)
   (at level 40).
 
-Record Guar {T A} (i : Name T)
-  (s : InterState (F A) (VE T A)) (x : Poss (VF T A))
-  (t : InterState (F A) (VE T A)) (y : Poss (VF T A))
+Record Inv {T A}
+  (s : InterState (F A) (VE T A)) (ρs : PossSet (VF T A))
 := {
-  increasing : snapSt x ⊆ snapSt y;
-  call_pres : forall j, i <> j -> PCalls x j = PCalls y j;
-  ret_pres : forall j, i <> j -> PRets x j = PRets y j
+  snap_cons :
+    ∀ ρ, ρs ρ ->
+      ∀ v, (∃ i, valSt s i = Some v) <-> v ∈ snapSt ρ;
+  rans_cons :
+    ∀ ρ, ρs ρ ->
+      ∀ i, uranSt s i = oranSt ρ i
+}.
+
+Record FillNewInv {T A} (i : Name T) (v : A) (vs : set A) (n : nat) (x : loop_st A)
+  (s : InterState (F A) (VE T A)) (ρs : PossSet (VF T A))
+:= {
+  fn_inv : Inv s ρs;
+  old_subs :
+    x.(old) ⊆ vs;
+  subs_new :
+    (λ v, v ∈ vs /\ ∃ i, `i ≥ n /\ valSt s i = Some v) ⊆ x.(new);
+  pfx_subs :
+    vs ⊆ (λ v, ∃ i, valSt s i = Some v);
+  poss_class :
+    ∀ ρ, ρs ρ ->
+      Waiting i (WriteSnap v) ρ \/ Done i (WriteSnap v) (Some vs) ρ;
+  poss_wait :
+    ∃ ρ, ρs ρ /\
+      Waiting i (WriteSnap v) ρ;
+  poss_done :
+    ∃ ρ, ρs ρ /\
+      Done i (WriteSnap v) (Some vs) ρ;
+}.
+
+Record Precs {T A} (i : Name T) (v : A)
+  (s : InterState (F A) (VE T A)) (ρs : PossSet (VF T A))
+:= {
+  ps_inv : Inv s ρs;
+  ps_wait : ∀ ρ, ρs ρ -> Waiting i (WriteSnap v) ρ
+}.
+
+Record Posts {T A} (i : Name T) (v : A) (r : option (set A))
+  (s : InterState (F A) (VE T A)) (ρs : PossSet (VF T A))
+:= {
+  qs_precs_hold : Precs i v s ρs;
+  qs_call_done : ∀ ρ, ρs ρ -> PCalls ρ i = CallDone (WriteSnap v);
+  qs_ret_done : ∀ ρ, ρs ρ -> PRets ρ i = RetPoss (WriteSnap v) r
 }.
 
 Record Rely {T A} (i : Name T)
-  (s : InterState (F A) (VE T A)) (x : Poss (VF T A))
-  (t : InterState (F A) (VE T A)) (y : Poss (VF T A))
+  (s : InterState (F A) (VE T A)) (ρs : PossSet (VF T A))
+  (t : InterState (F A) (VE T A)) (σs : PossSet (VF T A))
 := {
-  increases : snapSt x ⊆ snapSt y;
-  call_stay : PCalls x i = PCalls y i;
-  ret_stay : PRets x i = PRets y i
+
 }.
 
-Record Inv {T A}
-  (s : InterState (F A) (VE T A)) (x : Poss (VF T A))
+Record Guar {T A} (i : Name T)
+  (s : InterState (F A) (VE T A)) (ρs : PossSet (VF T A))
+  (t : InterState (F A) (VE T A)) (σs : PossSet (VF T A))
 := {
-  consistent :
-    forall v, (exists i, valSt s i = Some v) <-> v ∈ snapSt x
+
 }.
 
-Record InvW {T A} (i : Name T) (v : A)
-  (ls : loop_st A)
-  (s : InterState (F A) (VE T A)) (x : Poss (VF T A))
-  (b : bool)
-:= {
-  inv_holds : Inv s x;
-  old_sub : ls.(old) ⊆ snapSt x;
-  poss_status :
-    if b then
-      Waiting i (WriteSnap v) x
-    else
-      Done i (WriteSnap v) (Some ls.(new)) x
-}.
+Lemma fill_new_inv_stable {T A} {i : Name T} :
+  ∀ v vs n x,
+  Stable (Rely i) (FillNewInv (A:=A) i v vs n x).
+Proof.
+Admitted.
+
+Lemma fill_old_correct {T A} (i : Name T) (v : A) (x : loop_st A) :
+  VerifyProg i (Rely i) (Guar i)
+    (λ _ _, Precs i v)
+    (fill_old T x)
+    (λ '(tt, y) _ _ s ρs, ∃ vs, FillNewInv i v vs T y s ρs).
+Proof.
+Admitted.
+
+Lemma fill_new_correct {T A} (i : Name T) (v : A) (x : loop_st A) :
+  VerifyProg i (Rely i) (Guar i)
+    (λ _ _ s ρs, ∃ vs, FillNewInv i v vs T x s ρs)
+    (fill_new T x)
+    (λ '(tt, y) _ _ s ρs, ∃ vs, FillNewInv i v vs 0 y s ρs).
+Proof.
+  unfold fill_new.
+  unfold runStateM, bindM. simpl.
+  eapply weakenPost.
+  apply lemRange with
+    (I:=λ n x _ _ s ρs,
+      ∃ vs, FillNewInv i v vs n x s ρs);
+  clear.
+  2: now destruct v0, u.
+  intros n x Hlt.
+  unfold runStateM, bindM, lift.
+  simpl.
+  eapply lemBind with
+    (Q:=λ '(_, x'') _ _ s ρs,
+      ∃ vs, FillNewInv i v vs n x'' s ρs).
+  {
+    eapply lemBind.
+    {
+      apply (lemCall
+        (Q:=λ _ _ s ρs,
+          ∃ vs, FillNewInv i v vs (S n) x s ρs)
+        (S:=λ lsp _ _ s ρs,
+          ∃ vs, FillNewInv i v vs n x s ρs)).
+      {
+        unfold
+          Stable, stableRelt,
+          sub, subRelt.
+        intros. psimpl. exists x2.
+        apply fill_new_inv_stable.
+        psplit. exact H. easy.
+      }
+      {
+        unfold
+          Stable, stablePost, stableRelt,
+          sub, subRelt.
+        intros. psimpl. exists x2.
+        apply fill_new_inv_stable.
+        psplit. exact H. easy.
+      }
+      { admit. }
+      { admit. }
+    }
+    {
+      intros [val ran].
+      eapply lemRet.
+      unfold sub, subRelt.
+      intros. psimpl.
+      now exists x4.
+    }
+  }
+  intros [[val ran] x'].
+  unfold get, put. simpl.
+  rewrite ret_lunit.
+  destruct val; simpl.
+  {
+    apply lemRet.
+    unfold sub, subRelt.
+    intros _ _ s ρs [vs H].
+    exists vs. destruct H.
+    constructor; try easy.
+    {
+      intros. simpl.
+      apply subs_new0 in H.
+      now right.
+    }
+  }
+  { now apply lemRet. }
+Admitted.
+
 
 Lemma ws_correct {T A} (i : Name T) (v : A) :
-  VerifyProg i (LiftSRelt (Rely i)) (LiftSRelt (Guar i))
-      (prComp
-        (LiftSPrec Inv)
-        (TInvoke (snapImpl T A) i _ (WriteSnap v)) ->>
-        LiftSRelt (Rely i))
-      (write_snapshot v)
-      (fun _ _ _ => LiftSPrec Inv).
+  VerifyProg i (Rely i) (Guar i)
+    (prComp Inv (TInvoke (snapImpl T A) i _ (WriteSnap v)) ->> Rely i)
+    (write_snapshot v)
+    (λ r _ _, Posts i v r).
+Proof.
+  unfold write_snapshot.
+  apply lemBindSelf.
+  { admit. }
+  eapply lemBind.
+  {
+    admit.
+  }
+  intros i'.
+  eapply lemBind.
+  {
+    admit.
+  }
+  intros [val ran]. simpl.
+  destruct ran.
+  {
+    admit.
+  }
+  {
+    eapply lemBind with
+      (Q:=λ _ _ _, Precs i v).
+    {
+      admit.
+    }
+    intros [].
+    eapply lemBind.
+    {
+      unfold runStateM, bindM.
+      eapply lemBind.
+      { apply fill_old_correct. }
+      intros [[] [val' ran]].
+      eapply lemBind.
+      { apply fill_new_correct. }
+      intros [[] [val'' ran']].
+      eapply lemBind.
+    }
+  }
