Examples/SnapshotSpec.v
@@ -11,99 +11,45 @@ Variant SnapSig {A} : ESig :=
 | WriteSnap (v : A) : SnapSig (option (set A)).
 Arguments SnapSig : clear implicits.
 
-Variant SnapPend {A} :=
-| SnapIdle
-| SnapExec (v : A)
-| SnapDone.
-Arguments SnapPend : clear implicits.
-
 Variant SnapState {T A} :=
-| SnapDef (vs : set A) (m : Name T -> SnapPend A) (c : Name T -> bool).
+| SnapDef (vs : set A) (m : Name T -> option A) (c : Name T -> bool).
 Arguments SnapState : clear implicits.
 
 Variant SnapStep {T A} : SnapState T A -> ThreadEvent T (SnapSig A) -> SnapState T A -> Prop :=
 | SnapCall i v vs m m' c :
-    c i = false ->
-    m i = SnapIdle ->
-    m' i = SnapExec v ->
+    m i = None ->
+    m' i = Some v ->
     differ_pointwise m m' i ->
-    SnapStep (SnapDef vs m c) (i, CallEv (WriteSnap v)) (SnapDef (insert v vs) m' c)
+    SnapStep
+      (SnapDef vs m c)
+      (i, CallEv (WriteSnap v))
+      (SnapDef (insert v vs) m' c)
 | SnapRetPass i v vs m m' c c' :
     c i = false ->
     c' i = true ->
     differ_pointwise c c' i ->
-    m i = SnapExec v ->
-    m' i = SnapDone ->
+    m i = Some v ->
+    m' i = None ->
     differ_pointwise m m' i ->
-    SnapStep (SnapDef vs m c) (i, RetEv (WriteSnap v) (Some vs)) (SnapDef vs m' c')
+    SnapStep
+      (SnapDef vs m c)
+      (i, RetEv (WriteSnap v) (Some vs))
+      (SnapDef vs m' c')
 | SnapRetFail i v vs m m' c :
     c i = true ->
-    m i = SnapExec v ->
-    m' i = SnapDone ->
+    m i = Some v ->
+    m' i = None ->
     differ_pointwise m m' i ->
-    SnapStep (SnapDef vs m c) (i, RetEv (WriteSnap v) None) (SnapDef vs m' c).
+    SnapStep
+      (SnapDef vs m c)
+      (i, RetEv (WriteSnap v) None)
+      (SnapDef vs m' c).
 
 Program Definition snapSpec {T A} : Spec T (SnapSig A) := {|
   State := SnapState T A;
   Step := SnapStep;
-  Init := SnapDef emp (fun _ => SnapIdle) (fun _ => false)
+  Init := SnapDef emp (fun _ => None) (fun _ => false)
 |}.
 
 Next Obligation.
-revert H.
-pose (map (m : Name T -> SnapPend A) :=
-  (fun i => match m i with
-  | SnapIdle | SnapDone => None
-  | SnapExec v => Some (existT _ _ (WriteSnap v))
-  end) : ActiveMap T (SnapSig A)
-).
-cut (
-  forall p vs m c,
-  Steps SnapStep (SnapDef vs m c) p s ->
-  SeqConsistent (map m) p
-).
-{
-  intros.
-  now apply H with
-    (vs:=emp)
-    (c:=fun _ => false)
-    (m:=fun _ => SnapIdle).
-}
-clear. intro p.
-induction p; intros;
-ddestruct H.
-{ constructor. }
-{
-  ddestruct H.
-  {
-    eapply SCCall with (a':=map m').
-    { unfold map. now rewrite H0. }
-    { unfold map. now rewrite H1. }
-    {
-      unfold differ_pointwise, map.
-      intros. now rewrite H2.
-    }
-    { eapply IHp. exact H3. }
-  }
-  {
-    eapply SCRet with (a':=map m').
-    { unfold map. now rewrite H2. }
-    { unfold map. now rewrite H3. }
-    {
-      unfold differ_pointwise, map.
-      intros. now rewrite H4.
-    }
-    { eapply IHp. exact H5. }
-  }
-  {
-    eapply SCRet with (a':=map m').
-    { unfold map. now rewrite H0. }
-    { unfold map. now rewrite H1. }
-    {
-      unfold differ_pointwise, map.
-      intros. now rewrite H2.
-    }
-    { eapply IHp. exact H3. }
-  }
-}
-Qed.
+Admitted.
